theories/BasicAst.v
@@ -1,6 +1,4 @@
 (** * LogRel.BasicAst: definitions preceding those of the AST of terms: sorts, binder annotations… *)
-From Coq Require Import String Bool.
-From LogRel.AutoSubst Require Import core unscoped.
 
 Inductive sort : Set :=
   | set : sort.
