theories/Decidability/UntypedFunctions.v
@@ -1,0 +1,248 @@
+(** * LogRel.Decidability.UnytpedFunctions: implementation of untyped conversion. *)
+From Coq Require Import Nat Lia.
+From Equations Require Import Equations.
+From LogRel.AutoSubst Require Import core unscoped Ast Extra.
+From LogRel Require Import Utils BasicAst Context.
+From PartialFun Require Import Monad PartialFun.
+From LogRel.Decidability Require Import Functions.
+
+Import MonadNotations.
+Set Universe Polymorphism.
+Import IndexedDefinitions.
+
+
+#[local]Instance ty_errors : Errors := errors.
+#[local]Existing Instance MonadId | 10.
+#[local]Existing Instance MonadError | 1.
+
+Inductive nf_view2 : term -> term -> Type :=
+| sorts (s1 s2 : sort) : nf_view2 (tSort s1) (tSort s2)
+| prods (A A' B B' : term) :
+    nf_view2 (tProd A B) (tProd A' B')
+| nats : nf_view2 tNat tNat
+| emptys : nf_view2 tEmpty tEmpty
+| sigs (A A' B B' : term) : nf_view2 (tSig A B) (tSig A' B')
+| ids A A' x x' y y' : nf_view2 (tId A x y) (tId A' x' y')
+| lams A A' t t' : nf_view2 (tLambda A t) (tLambda A' t')
+| lam_ne A t n' : nf_view2 (tLambda A t) n'
+| ne_lam n A' t' : nf_view2 n (tLambda A' t')
+| zeros : nf_view2 tZero tZero
+| succs t t' : nf_view2 (tSucc t) (tSucc t')
+| pairs A A' B B' t t' u u' :
+    nf_view2 (tPair A B t u) (tPair A' B' t' u')
+| pair_ne A B t u n' :
+    nf_view2 (tPair A B t u) n'
+| ne_pair n A' B' t' u' :
+    nf_view2 n (tPair A' B' t' u')
+| refls A A' x x' : nf_view2 (tRefl A x) (tRefl A' x')
+| neutrals (n n' : term) : nf_view2 n n'
+| mismatch (t u : term) : nf_view2 t u
+| anomaly (t u : term) : nf_view2 t u.
+
+Equations build_nf_view2 (t t' : term) : nf_view2 t t' :=
+  build_nf_view2 t t' with (build_nf_view1 t) := {
+  | nf_view1_type (eSort s) with (build_nf_view1 t') := {
+    | nf_view1_type (eSort s') := sorts s s' ;
+    | nf_view1_type _ := mismatch _ _ ;
+    | nf_view1_ne _ := mismatch _ _ ;
+    | _ := anomaly _ _ } ;
+  | nf_view1_type (eProd A B) with (build_nf_view1 t') := {
+    | nf_view1_type (eProd A' B') := prods A A' B B' ;
+    | nf_view1_type _ := mismatch _ _ ;
+    | nf_view1_ne _ := mismatch _ _ ;
+    | _ := anomaly _ _ } ;
+  | nf_view1_type eNat with (build_nf_view1 t') := {
+    | nf_view1_type eNat := nats ;
+    | nf_view1_type _ := mismatch _ _ ;
+    | nf_view1_ne _ := mismatch _ _ ;
+    | _ := anomaly _ _ } ;
+  | nf_view1_type eEmpty with (build_nf_view1 t') := {
+    | nf_view1_type eEmpty := emptys ;
+    | nf_view1_type _ := mismatch _ _ ; 
+    | _ := anomaly _ _ } ;
+  | nf_view1_type (eSig A B) with (build_nf_view1 t') := {
+    | nf_view1_type (eSig A' B') := sigs A A' B B' ;
+    | nf_view1_type _ := mismatch _ _ ;
+    | nf_view1_ne _ := mismatch _ _ ;
+    | _ := anomaly _ _ } ;
+  | nf_view1_type (eId A x y) with (build_nf_view1 t') := {
+    | nf_view1_type (eId A' x' y') := ids A A' x x' y y' ;
+    | nf_view1_type _ := mismatch _ _ ;
+    | nf_view1_ne _ := mismatch _ _ ;
+    | _ := anomaly _ _ } ;
+  | nf_view1_fun A t with (build_nf_view1 t') := {
+    | nf_view1_fun A' t' := lams A A' t t' ;
+    | nf_view1_ne _ := lam_ne A t _ ; 
+    | _ := anomaly _ _ } ;
+  | nf_view1_nat eZero with (build_nf_view1 t') := {
+    | nf_view1_nat eZero := zeros ;
+    | nf_view1_nat (eSucc _) := mismatch _ _ ;
+    | nf_view1_ne _ := mismatch _ _ ; 
+    | _ := anomaly _ _ } ;
+  | nf_view1_nat (eSucc u) with (build_nf_view1 t') := {
+    | nf_view1_nat (eSucc u') := succs u u' ;
+    | nf_view1_nat eZero := mismatch _ _ ;
+    | nf_view1_ne _ := mismatch _ _ ; 
+    | _ := anomaly _ _ } ;
+  | nf_view1_sig A B t u with (build_nf_view1 t') := {
+    | nf_view1_sig A' B' t' u' := pairs A A' B B' t t' u u' ;
+    | nf_view1_ne _ := pair_ne A B t u _ ; 
+    | _ := anomaly _ _ } ;
+  | nf_view1_id A x with (build_nf_view1 t') := {
+    | nf_view1_id A' x' := refls A A' x x' ;
+    | nf_view1_ne _ := mismatch _ _ ;
+    | _ := anomaly _ _ } ;
+  | nf_view1_ne _ with (build_nf_view1 t') := {
+    | nf_view1_type _ := mismatch _ _ ;
+    | nf_view1_fun A' t' := ne_lam _ A' t' ;
+    | nf_view1_nat _ := mismatch _ _ ;
+    | nf_view1_sig A' B' t' u' := ne_pair _ A' B' t' u' ;
+    | nf_view1_id _ _ := mismatch _ _ ;
+    | nf_view1_ne _ := neutrals _ _ ;
+  }
+  }.
+
+  Variant uconv_state : Type :=
+  | ty_state (** Conversion of arbitrary types *)
+  | ty_red_state (** Comparison of types in weak-head normal forms *)
+  | tm_state (** Conversion of arbitrary terms *)
+  | tm_red_state (** Comparison of terms if weak-head normal forms *)
+  | ne_state. (** Comparison of neutrals *)
+
+Section Conversion.
+
+Definition uconv_dom := uconv_state × term × term.
+Definition uconv_cod (_ : uconv_dom) := result unit.
+
+#[local] Instance: forall x, PFun (singleton_store wh_red x) := singleton_pfun wh_red.
+
+#[local]
+Notation M0 := (irec (singleton_store wh_red) (uconv_dom) (uconv_cod)).
+#[local]
+Notation M := (errrec (singleton_store wh_red) (A:=uconv_dom) (B:=uconv_cod)).
+
+#[local] Instance: Monad M0 := MonadOrec.
+#[local] Instance: Monad M := monad_erec.
+
+Equations uconv_ty :
+  (term × term) -> M unit :=
+  | (T,V) :=
+    T' ← call_single wh_red T ;;[M0]
+    V' ← call_single wh_red V ;;[M0]
+    id <*> rec (ty_red_state,T',V').
+
+Equations uconv_ty_red : 
+  (term × term) -> M unit :=
+  | (T,T') with (build_nf_ty_view2 T T') :=
+  {
+    | ty_sorts s s' := ret (eq_sort s s') ;
+    | ty_prods A A' B B' :=
+        rec (ty_state,A,A') ;;
+        rec (ty_state,B,B') ;
+    | ty_nats := success ;
+    | ty_emptys := success ;
+    | ty_sigs A A' B B' :=
+        rec (ty_state,A,A') ;;
+        rec (ty_state,B,B') ;
+      | ty_neutrals _ _ :=
+          rec (ne_state,T,T') ;
+    | ty_ids A A' x x' y y' :=
+      rec (ty_state,A,A') ;;
+      rec (tm_state,x,x') ;;
+      rec (tm_state,y,y') ;
+    | ty_mismatch _ _ := raise (head_mismatch None T T') ;
+    | ty_anomaly _ _ := undefined ;
+  }.
+
+Equations uconv_tm : (term × term) -> M unit :=
+  | (t,u) :=
+    t' ← call_single wh_red t ;;[M0]
+    u' ← call_single wh_red u ;;[M0]
+    id <*> rec (tm_red_state,t',u').
+    
+Equations uconv_tm_red : (term × term) -> M unit :=
+  | (t,t') with (build_nf_view2 t t') :=
+  {
+    | sorts s s' :=
+        ret (eq_sort s s') ;
+    | prods A A' B B' :=
+        rec (tm_state,A,A') ;;
+        rec (tm_state,B,B') ;
+    | nats := success ;
+    | emptys := success ;
+    | sigs A A' B B' :=
+        rec (tm_state,A,A') ;;
+        rec (tm_state,B,B') ;
+    | ids A A' x x' y y' :=
+        rec (tm_state,A,A') ;;
+        rec (tm_state,x,x') ;;
+        rec (tm_state,y,y') ;
+    | lams _ _ t t' :=
+        rec (tm_state,t,t') ;
+    | lam_ne _ t t' :=
+        rec (tm_state,t,eta_expand t') ;
+    | ne_lam t _ t' :=
+        rec (tm_state,eta_expand t,t') ;
+    | zeros := success ;
+    | succs t t' :=
+        rec (tm_state,t,t') ;
+    | pairs _ _ _ _ t t' u u' :=
+        rec (tm_state,t,t') ;;
+        rec (tm_state,u,u') ;
+    | pair_ne _ _ t u t' :=
+        rec (tm_state,t,tFst t') ;;
+        rec (tm_state,u,tSnd t') ;
+    | ne_pair t _ _ t' u' :=
+        rec (tm_state,tFst t, t') ;;
+        rec (tm_state,tSnd t,u') ;
+    | refls A A' x x' := 
+      rec (ty_state,A,A') ;;
+      rec (tm_state,x,x') ;
+    | neutrals _ _ :=
+      rec (ne_state,t,t') ;
+    | mismatch _ _ := raise (head_mismatch None t t') ;
+    | anomaly _ _ := undefined ;
+  }.
+
+Equations uconv_ne : (term × term) -> M unit :=
+  | (tRel n , tRel n')
+      with n =? n' :=
+      { | false := raise (variable_mismatch n n') ;
+        | true := success ;
+      } ;
+      
+  | (tApp n t , tApp n' t') :=
+    rec (ne_state,n,n') ;;
+    rec (tm_state,t,t') ;
+
+| (tNatElim P hz hs n,tNatElim P' hz' hs' n') :=
+  rec (ne_state,n,n') ;;
+  rec (ty_state,P,P') ;;
+  rec (tm_state,hz,hz') ;;
+  rec (tm_state,hs,hs')
+
+| (tEmptyElim P n,tEmptyElim P' n') :=
+  rec (ne_state,n,n') ;;
+  rec (ty_state,P,P')
+
+| ( tFst n , tFst n') :=
+  rec (ne_state,n,n')
+
+| ( tSnd n , tSnd n') :=
+  rec (ne_state,n,n')
+
+| (n,n') := raise (destructor_mismatch n n').
+
+Equations _conv : (uconv_state × term × term) ⇀[singleton_store wh_red] result unit :=
+  | (ty_state,ts) := uconv_ty ts;
+  | (ty_red_state,ts) := uconv_ty_red ts ;
+  | (tm_state,ts) := uconv_tm ts ;
+  | (tm_red_state,ts) := uconv_tm_red ts;
+  | (ne_state,ts) := uconv_ne ts.
+
+  Import StdInstance.
+
+  Equations uconv : (context × term × term) ⇀ result unit :=
+    uconv (Γ,T,V) := call _conv (ty_state,T,V).
+  
+End Conversion.
